thys/Native_Word/Uint64.thy
@@ -493,7 +493,7 @@ lemma Uint64_code [code]:
 lemma Uint64_signed_code [code]:
   "Rep_uint64 (Uint64_signed i) = 
   (if i < -(0x8000000000000000) \<or> i \<ge> 0x8000000000000000 then Rep_uint64 (undefined Uint64 i) else word_of_int (int_of_integer_symbolic i))"
-unfolding Uint64_signed_def Uint64_def int_of_integer_symbolic_def word_of_integer_def
+unfolding Uint64_signed_def Uint64_def int_of_integer_symbolic_def
 by(simp add: Abs_uint64_inverse)
 
 end
